Tap

FreydSSA/Ctx/Var/Ix.lean
@@ -4,88 +4,198 @@ import FreydSSA.Ctx.Var.Fun
 variable {ν ν' α β} [DecidableEq ν] [DecidableEq ν'] [DecidableEq α]
 
 structure TCtx (α : Type v) : Type _ where
-  arity : ℕ
-  ty : Fin arity → α
+  length : ℕ
+  ty : Fin length → α
+
+def TCtx.nil : TCtx α := ⟨0, λi => i.elim0⟩
+def TCtx.cons (A : α) (Γ : TCtx α) : TCtx α := ⟨Γ.length + 1, Fin.cons A Γ.ty⟩
+
+--TODO: get extensionality
+
+theorem TCtx.length_zero_eq_nil {Γ : TCtx α} (h : Γ.length = 0) : Γ = TCtx.nil := by
+  cases Γ
+  cases h
+  simp only [nil, mk.injEq, heq_eq_eq, true_and] at *
+  funext i
+  exact i.elim0
+
+theorem TCtx.length_zero_eq {Γ Δ : TCtx α} (hΓ : Γ.length = 0) (hΔ : Δ.length = 0) : Γ = Δ
+  := Γ.length_zero_eq_nil hΓ ▸ Δ.length_zero_eq_nil hΔ ▸ rfl
+
+def TCtx.append (Γ Δ : TCtx α) : TCtx α := ⟨Γ.length + Δ.length, Fin.append Γ.ty Δ.ty⟩
+
+def TCtx.fromList : List α → TCtx α
+  | [] => TCtx.nil
+  | A :: Γ => TCtx.cons A (TCtx.fromList Γ)
+
+def TCtx.toList : TCtx α → List α
+  | ⟨0, _⟩ => []
+  | ⟨n+1, ty⟩ => ty 0 :: TCtx.toList ⟨n, λi => ty i.succ⟩
+
+theorem TCtx.toList_fromList (Γ : List α) : (TCtx.fromList Γ).toList = Γ := by
+  induction Γ with
+  | nil => rfl
+  | cons A Γ I =>
+    simp only [toList, fromList, cons]
+    congr 1
+
+theorem TCtx.fromList_toList : (Γ : TCtx α) → TCtx.fromList Γ.toList = Γ := by
+  intro ⟨n, Γi⟩
+  induction n with
+  | zero => exact length_zero_eq rfl rfl
+  | succ n I =>
+    simp only [toList]
+    rw [fromList, cons, I]
+    simp only [mk.injEq, heq_eq_eq, true_and]
+    funext ⟨i, hi⟩
+    cases i <;> rfl
+
+theorem TCtx.toList_length : (Γ : TCtx α) → Γ.toList.length = Γ.length := by
+  intro ⟨n, Γi⟩
+  induction n with
+  | zero => rfl
+  | succ n I =>
+    simp only [toList]
+    rw [List.length_cons, I]
+
+theorem TCtx.fromList_length (Γ : List α) : (TCtx.fromList Γ).length = Γ.length := by
+  induction Γ with
+  | nil => rfl
+  | cons A Γ I =>
+    simp only [fromList, cons, length]
+    rw [I]
+    rfl
+
+def TCtx.map (f : α → β) (Γ : TCtx α) : TCtx β := ⟨Γ.length, f ∘ Γ.ty⟩
+
+theorem TCtx.fromList_map {f : α → β} (Γ : List α) : (TCtx.fromList (Γ.map f)) = (TCtx.fromList Γ).map f := by
+  induction Γ with
+  | nil => exact length_zero_eq rfl rfl
+  | cons A Γ I =>
+    simp only [fromList, map, cons, mk.injEq, heq_eq_eq, true_and, I]
+    funext ⟨i, hi⟩
+    cases i <;> rfl
+
+theorem TCtx.toList_map {f : α → β} : (Γ : TCtx α) → (Γ.map f).toList = Γ.toList.map f := by
+  intro ⟨n, Γi⟩
+  induction n with
+  | zero => rfl
+  | succ n I =>
+    simp only [toList, map]
+    rw [List.map, <-I]
+    rfl
 
 structure ICtx (ν : Type u) (α : Type v) extends TCtx α : Type (max u v) where
-  name : Fin arity → ν
+  name : Fin length → ν
+
+def ICtx.map (f: α → β) (Γ : ICtx ν α) : ICtx ν β := ⟨Γ.toTCtx.map f, Γ.name⟩
+def ICtx.map_names (f : ν → ν') (Γ : ICtx ν α) : ICtx ν' α := ⟨Γ.toTCtx, f ∘ Γ.name⟩
+
+--TODO: ICtx ≅ Ctx
+--TODO: TCtx iso preservation...
 
 structure IFCtx (ν : Type u) (α : Type v) extends ICtx (WithBot ν) α : Type (max u v) where
   no_shadow : ∀ i j, name i = name j -> name i = ⊥ ∨ i = j
 
+def IFCtx.map (f: α → β) (Γ : IFCtx ν α) : IFCtx ν β := ⟨Γ.toICtx.map f, Γ.no_shadow⟩
+--TODO: IFCtx name mapping
+
 structure ISCtx (ν : Type u) (α : Type v) extends ICtx ν α : Type (max u v) where
-  nodup : ∀ i j, name i = name j -> i = j
+  nodup : Function.Injective name
+
+def ISCtx.map (f: α → β) (Γ : ISCtx ν α) : ISCtx ν β := ⟨Γ.toICtx.map f, Γ.nodup⟩
+--TODO: ISCtx name mapping
 
 structure FICtx (ν : Type u) (α : Type v) extends TCtx α : Type (max u v) where
-  ix : FCtx ν (Fin arity)
+  ix : FCtx ν (Fin length)
   injective : Function.Injective ix
 
---TODO: ICtx ≅ Ctx
+def FICtx.map (f: α → β) (Γ : FICtx ν α) : FICtx ν β := ⟨Γ.toTCtx.map f, Γ.ix, Γ.injective⟩
+--TODO: FICtx name mapping
 
 --TODO: map functions, positional map functions
 
 --TODO: ICtx → (IFCtx, FICtx)
 
 --TODO: FICtx ≅ IFCtx, TCtx equal...
+--TODO: ISCtx → IFCtx via map_names coe
 
-def TCtx.Var {α} (Γ : TCtx α) (A : α) (i : Fin Γ.arity) : Prop := Γ.ty i = A
+def TCtx.Var (Γ : TCtx α) (A : α) (i : Fin Γ.length) : Prop := Γ.ty i = A
 
 --TODO: factor out ix for Wk variants? can then use subset types...
 
-structure TCtx.Wk {α} (Γ : TCtx α) (Δ : TCtx α) (ρ : Fin Δ.arity → Fin Γ.arity) : Prop where
+structure TCtx.Wk (Γ : TCtx α) (Δ : TCtx α) (ρ : Fin Δ.length → Fin Γ.length) : Prop where
   ty_eq : ∀i, Γ.ty (ρ i) = Δ.ty i
   injective : Function.Injective ρ
 
-structure ICtx.Var {ν α} (Γ : ICtx ν α) (x : ν) (A : α) (i : Fin Γ.arity) : Prop where
+theorem TCtx.id (Γ : TCtx α) : TCtx.Wk Γ Γ id where
+  ty_eq _ := rfl
+  injective := Function.injective_id
+
+theorem TCtx.comp {Γ Δ Ξ : TCtx α} {ρ σ} (hρ : TCtx.Wk Γ Δ ρ) (hσ : TCtx.Wk Δ Ξ σ) : TCtx.Wk Γ Ξ (ρ ∘ σ) where
+  ty_eq i := by rw [Function.comp, hρ.ty_eq, hσ.ty_eq]
+  injective := hρ.injective.comp hσ.injective
+
+theorem TCtx.Var.wk {Γ Δ : TCtx α} {ρ A i} (hρ : TCtx.Wk Γ Δ ρ) (h : Δ.Var A i) : Γ.Var A (ρ i)
+  := (hρ.ty_eq i).trans h
+
+structure ICtx.Var (Γ : ICtx ν α) (x : ν) (A : α) (i : Fin Γ.length) : Prop where
   ix_name : Γ.name i = x
   ix_ty : Γ.ty i = A
   ix_last : ∀j, Γ.name j = x → j ≤ i
 
-structure IFCtx.Var {ν α} (Γ : IFCtx ν α) (x : ν) (A : α) (i : Fin Γ.arity) : Prop where
+structure IFCtx.Var (Γ : IFCtx ν α) (x : ν) (A : α) (i : Fin Γ.length) : Prop where
   ix_name : Γ.name i = x
   ix_ty : Γ.ty i = A
 
 --TODO: IFCtx.Var ↔ ICtx.Var (using toICtx)
 
-structure FICtx.Var {ν α} (Γ : FICtx ν α) (x : ν) (A : α) (i : Fin Γ.arity) : Prop where
+structure ISCtx.Var (Γ : ISCtx ν α) (x : ν) (A : α) (i : Fin Γ.length) extends Γ.toICtx.Var x A i : Prop where
+  ix_last _ hj := le_of_eq (Γ.nodup (hj.trans ix_name.symm))
+
+--TODO: nicer constructors?
+
+structure FICtx.Var (Γ : FICtx ν α) (x : ν) (A : α) (i : Fin Γ.length) : Prop where
   ix_name : Γ.ix x = i
   ix_ty : Γ.ty i = A
 
 -- *syntactic* weakening, in which shadowed variables are simply ignored
-structure ICtx.VWk {ν α} (Γ : ICtx ν α) (Δ : ICtx ν α) where
-  ix : Fin Δ.arity → Fin Γ.arity
-  var : ∀{x A i}, Δ.Var x A i → Γ.Var x A (ix i)
+def ICtx.VWk (Γ : ICtx ν α) (Δ : ICtx ν α) (ρ : Fin Δ.length → Fin Γ.length) := ∀{x A i}, Δ.Var x A i → Γ.Var x A (ρ i)
 
 -- *semantic* weakening, which can be interpreted nicely for affine variables
 -- Note that the _names_ of shadowed variables don't matter
-structure ICtx.Wk {ν α} (Γ : ICtx ν α) (Δ : ICtx ν α) (ρ : Fin Δ.arity → Fin Γ.arity) extends TCtx.Wk Γ.toTCtx Δ.toTCtx ρ : Prop where
+structure ICtx.Wk (Γ : ICtx ν α) (Δ : ICtx ν α) (ρ : Fin Δ.length → Fin Γ.length) extends TCtx.Wk Γ.toTCtx Δ.toTCtx ρ : Prop where
   var : ∀{x A i}, Δ.Var x A i → Γ.Var x A (ρ i)
 
---TODO: ICtx.Wk --> ICtx.VWk, with equal indices
+theorem ICtx.Var.wk {Γ Δ : ICtx ν α} {ρ x A i} (hρ : ICtx.Wk Γ Δ ρ) (h : Δ.Var x A i) : Γ.Var x A (ρ i)
+  := hρ.var h
 
 -- *strict* weakening, which does not swap variables, and respects all variable names
-structure ICtx.SWk {ν α} (Γ : ICtx ν α) (Δ : ICtx ν α) (ρ : Fin Δ.arity → Fin Γ.arity) extends Wk Γ Δ ρ : Prop where
+structure ICtx.SWk (Γ : ICtx ν α) (Δ : ICtx ν α) (ρ : Fin Δ.length → Fin Γ.length) extends Wk Γ Δ ρ : Prop where
   name_eq : ∀i, Γ.name (ρ i) = Δ.name i
   monotone : Monotone ρ
 
---TODO: Strict weakning ≅ Ctx weakening
+-- theorem ICtx.SWk.wk_eq {Γ Δ : ICtx ν α} {ρ σ} (hρ : ICtx.SWk Γ Δ ρ) (hσ : ICtx.SWk Γ Δ σ) : ρ = σ := by
+--   funext i
+
+--TODO: Strict weakning ≅ Ctx weakening, or think about this...
 
 --TODO: Weakening _preorder_ on ICtx
 
 --TODO: Connection between FCtx and ICtx
 
-
 --TODO: ICtx comparability
 
-structure IFCtx.VWk {ν α} (Γ : IFCtx ν α) (Δ : IFCtx ν α) (ρ : Fin Δ.arity → Fin Γ.arity) extends TCtx.Wk Γ.toTCtx Δ.toTCtx ρ : Prop where
+structure IFCtx.VWk (Γ : IFCtx ν α) (Δ : IFCtx ν α) (ρ : Fin Δ.length → Fin Γ.length) extends TCtx.Wk Γ.toTCtx Δ.toTCtx ρ : Prop where
   var : ∀{x A i}, Δ.Var x A i → Γ.Var x A (ρ i)
 
-structure IFCtx.Wk {ν α} (Γ : IFCtx ν α) (Δ : IFCtx ν α) (ρ : Fin Δ.arity → Fin Γ.arity) extends TCtx.Wk Γ.toTCtx Δ.toTCtx ρ : Prop where
+structure IFCtx.Wk (Γ : IFCtx ν α) (Δ : IFCtx ν α) (ρ : Fin Δ.length → Fin Γ.length) extends TCtx.Wk Γ.toTCtx Δ.toTCtx ρ : Prop where
   name_eq : ∀i, Γ.name (ρ i) = Δ.name i
 
 --TODO: IFCtx.Wk --> IFCtx.VWk
 
-structure FICtx.Wk {ν α} (Γ : FICtx ν α) (Δ : FICtx ν α) (ρ : Fin Δ.arity → Fin Γ.arity) extends TCtx.Wk Γ.toTCtx Δ.toTCtx ρ : Prop where
-  name_eq : ∀x, (Δ.ix x).map ρ ⊆ Γ.ix x
+structure ISCtx.Wk (Γ : ISCtx ν α) (Δ : ISCtx ν α) (ρ : Fin Δ.length → Fin Γ.length) extends TCtx.Wk Γ.toTCtx Δ.toTCtx ρ : Prop where
+  name_eq : ∀i, Γ.name (ρ i) = Δ.name i
 
---TODO: likewise for IFCtx, FICtx, ISCtx, etc...
+structure FICtx.Wk (Γ : FICtx ν α) (Δ : FICtx ν α) (ρ : Fin Δ.length → Fin Γ.length) extends TCtx.Wk Γ.toTCtx Δ.toTCtx ρ : Prop where
+  name_eq : ∀x, (Δ.ix x).map ρ ⊆ Γ.ix x
